theories/weakestpre/specifications.v
@@ -9,11 +9,13 @@ From osiris.lang Require Import lang.
 From osiris.semantics Require Import semantics.
 From osiris.weakestpre Require Import wp wp_tactics.
 
+(* This file should move to the [proofmode] directory. *)
+
 
 
 (* The follwoing section defines the typeclasses to use to define a
    specification. *)
-Section TypeclassesDefinitions.
+Section FunctionSpecifications.
   Context `{!osirisGS_gen hlc Σ}.
 
   (* [pure_unary_spec] is used to tell osiris that [f] represents a closure
@@ -55,4 +57,180 @@ Section TypeclassesDefinitions.
                        φ vpartial) -∗ (* TODO: get a later here. *)
         wp s E (call f #a) φ.
 
-End TypeclassesDefinitions.
+End FunctionSpecifications.
+
+(* -------------------------------------------------------------------------- *)
+
+(* The following section provides helper lemmas to reason on mutually-recursive
+   functions ([let rec ... and ...] and [let ... = ...] constructs). *)
+Section MutuallyRecursive.
+
+  Context `{!osirisGS_gen hlc Σ}.
+
+  (* ------------------------------------------------------------------------ *)
+
+  (* The idea of this section is to allow to prove goals of the form
+     [wp s E (concatenating ...) φ] and [wp s E (dconcatenating ...) φ] by
+     proving that it is enough to prove:
+     [ ▷ spec1 v1 -∗ ... -∗ ▷ specn vn -∗ spec1 v1 ],
+      ... ,
+     [ ▷ spec1 v1 -∗ ... -∗ ▷ specn vn -∗ specn vn ], and
+     [ (spec1 v1 -∗ ... -∗ specn vn -∗ P) ],
+     where [P] represents the initial goal to prove.
+
+     Note: it does not seem possible to prove the lines above in separate
+           branches of the proof (ie. outside of the Iris proofmode) as one may
+           need resources to prove the specifications.
+           There does not seem to be an easy way to share the resources and keep
+           the built-in Löb induction. *)
+
+  (* ------------------------------------------------------------------------ *)
+
+  (* Definitions to build the lemmas on mutually-recursive functions. *)
+
+  Definition conjn (pl: list (iProp Σ)) : iProp Σ :=
+    foldr (fun e res => e ∗ res)%I emp%I pl.
+
+  Definition wandn (pl: list (iProp Σ)) (P: iProp Σ) : iProp Σ :=
+    foldr (fun e res => e -∗ res)%I P pl.
+
+  Definition sepn_wand (pl: list (iProp Σ)) (P: iProp Σ) : iProp Σ :=
+    conjn pl -∗ P.
+
+  Lemma wandn_sepn_wand_1 (pl: list (iProp Σ)) (P: iProp Σ) :
+    wandn pl P -∗ sepn_wand pl P.
+  Proof.
+    iInduction (pl) as [ | p pl ] "IH";
+      unfold wandn; unfold sepn_wand; simpl; auto.
+
+    iIntros "H_impl [Hp H_conj]".
+    iApply ("IH" with "[H_impl Hp] H_conj").
+    iApply ("H_impl" with "Hp").
+  Qed.
+
+  Lemma wandn_sepn_wand_2 (pl: list (iProp Σ)) (P: iProp Σ) :
+    sepn_wand pl P -∗ wandn pl P.
+  Proof.
+    iInduction (pl) as [ | p pl ] "IH";
+      unfold wandn; unfold sepn_wand; simpl.
+
+    { iIntros "H". iApply ("H" with "[//]"). }
+
+    iIntros "H_sepn Hp".
+    iPoseProof (wand_curry with "H_sepn Hp") as "H_sepn".
+    iApply ("IH" with "H_sepn").
+  Qed.
+
+  (* ------------------------------------------------------------------------ *)
+
+  Lemma conjn_later_1 (pl: list (iProp Σ)) :
+    ▷ conjn pl -∗ conjn (map (fun e => ▷ e)%I pl).
+  Proof.
+    iInduction pl as [ | p pl ] "IH"; simpl; auto.
+    iIntros "[$ Hpl]".
+    iApply ("IH" with "Hpl").
+  Qed.
+
+  Lemma conjn_later_2 (pl: list (iProp Σ)) :
+    conjn (map (fun e => ▷ e)%I pl) -∗ ▷ conjn pl.
+  Proof.
+    iInduction pl as [ | p pl ] "IH"; simpl; auto.
+    iIntros "[$ Hpl]".
+    iApply ("IH" with "Hpl").
+  Qed.
+
+  Lemma conjn_pers (pl: list (iProp Σ)) :
+    Forall Persistent pl →
+    Persistent (conjn pl).
+  Proof.
+    induction pl as [ | p pl IH].
+    { simpl. intros. apply emp_persistent. }
+
+    { intros [Hp Hpl]%Forall_cons.
+      simpl. apply sep_persistent; first exact Hp.
+      exact (IH Hpl). }
+  Qed.
+
+  Lemma conjn_löb pl :
+    (□ (conjn (map (fun e => ▷ e)%I pl) -∗ conjn pl)) -∗
+    conjn pl.
+  Proof.
+    iIntros "#H1".
+    iLöb as "Hl".
+    iApply "H1".
+    iApply (conjn_later_1 with "Hl").
+  Qed.
+
+  Lemma wand_conjn_l (pl: list (iProp Σ)) (P: iProp Σ) :
+    Persistent P →
+    conjn (map (fun p => P -∗ p) pl)%I -∗
+    (P -∗ conjn pl).
+  Proof.
+    intros Hpers.
+    iInduction (pl) as [ | p pl ] "IH"; auto; simpl.
+    iIntros "[Hp Hpl] #HP".
+    iPoseProof ("IH" with "Hpl HP") as "$".
+    iApply ("Hp" with "HP").
+  Qed.
+
+  Lemma persistent_intro (P: iProp Σ):
+    (Persistent P -> ⊢ P -∗ □ P)%I.
+  Proof. auto. Qed.
+
+  Lemma conjn_persistent_l (pl: list (iProp Σ)) :
+    conjn (map (λ e, □ e)%I pl) -∗ (□ conjn pl).
+  Proof.
+    iInduction (pl) as [ | p pl ] "IH"; auto; simpl.
+    assert (Persistent (conjn (map (λ e, □ e)%I pl))).
+    { apply conjn_pers. induction pl as [ | ? ? IHpl ]; simpl;
+        [ by apply Forall_nil | apply Forall_cons; split].
+      - apply intuitionistically_persistent.
+      - apply IHpl. }
+    iIntros "[#Hp #Hpl]".
+    iSplitL; first by auto.
+    iApply ("IH" with "Hpl").
+  Qed.
+
+  Lemma conjn_weaken2 (f g: iProp Σ → iProp Σ) (pl: list (iProp Σ)) :
+    (forall e, f e -∗ g e) → conjn (map f pl) -∗ conjn (map g pl).
+  Proof.
+    iIntros (Hf).
+    induction pl as [ | p pl IH ]; simpl; auto.
+    iIntros "[Hp Hpl]".
+    iSplitL "Hp".
+    { iApply (Hf with "Hp"). }
+    { iApply (IH with "Hpl"). }
+  Qed.
+
+  Lemma prove_specify (pl: list (iProp Σ)) (P: iProp Σ) :
+    Forall Persistent pl → ⊢
+    (*□ (wandn (map (fun e => ▷ e)%I pl) (conjn pl)) -∗*)
+    (wandn
+       (map (λ p, □ p)
+       (map (λ p, wandn (map (λ e : iPropI Σ, ▷ e) pl) p) pl)))%I
+    ((wandn pl P) -∗
+    P).
+  Proof.
+    intros Hpers.
+    iApply wandn_sepn_wand_2.
+    iIntros "Hspecs1 HP"; unfold sepn_wand.
+    iPoseProof (conjn_persistent_l with "Hspecs1") as "#Hspecs3".
+    iPoseProof (wandn_sepn_wand_1 with "HP") as "HP".
+    unfold sepn_wand.
+
+    assert (Persistent (conjn (map (λ e, ▷ e)%I pl))).
+    { apply conjn_pers.
+      induction pl as [ | p pl IH]; first by apply Forall_nil.
+      apply Forall_cons in Hpers as [Hp Hpl].
+      apply Forall_cons; split;
+        [ exact (later_persistent _ Hp)
+        | exact (IH Hpl) ]. }
+    iPoseProof (conjn_weaken2 with "Hspecs3") as "#Hspecs".
+    { iIntros (e) "H".
+      iApply (wandn_sepn_wand_1 with "H"). }
+    iPoseProof ((wand_conjn_l pl (conjn (map (λ e : iPropI Σ, ▷ e)%I pl))
+                              H) with "Hspecs") as "Hspecs2".
+    iPoseProof (conjn_löb with "Hspecs2") as "Hspecs4".
+    iApply ("HP" with "Hspecs4").
+  Qed.
+End MutuallyRecursive.
